Cleanup and WIP

Hoare_Triple.v
@@ -20,11 +20,7 @@ Definition postcondition : Type := sigma -> sigma -> Prop.
 
 Definition empty_postcondition :  postcondition := (fun _ _ => True).
 
-(** ------------------------------ **)
-(** Partial correcness             **)
-(** ------------------------------ **)
-
-(** Definition of functional correcness i.e Hoare Triples **)
+(** Definition of functional correcness / Hoare Triples / Partial correcness **)
 
 Definition hoare_triple (P : precondition) (Q: postcondition) (c : com) (ps : Psi.psi) : Prop :=
   forall s s',  P s -> ceval c s ps s' -> Q s' s.
@@ -65,19 +61,61 @@ Proof.
     + apply H6.
 Qed.
 
+Module SF.
+
+  Lemma while_triple :
+    forall (inv: assertion) (var: variant) b c ps l,
+      hoare_triple (fun s => inv (s :: l) /\ beval s b = true)
+        (fun s' _ => inv (s' :: l)) c ps ->
+      hoare_triple (fun s => inv (s :: l))
+        ( fun s' _ => inv (s' :: l) /\ beval s'  b = false )
+        (CWhile b c inv var) ps.
+  Proof.
+    intros P var b c ps l Hhoare st st' HP Heval.
+    remember (CWhile b c P var) as original_command eqn:Horig.
+    induction Heval; inversion Horig;subst;eauto.
+  Qed.
+
+End SF.
+
+Definition bi_hoare (i: nat) (P: precondition) (Q: postcondition)
+           (c : com) (b: bexp) (ps : Psi.psi) : Prop :=
+  forall s s', P s -> ceval (unroll i b c) s ps s' -> Q s' s.
+
+Lemma bi_uadruple_quadruple P Q p b inv var ps:
+  hoare_triple P Q (CWhile b p inv var) ps <->
+    forall n, bi_hoare n P Q p b ps.
+Proof.
+  unfold hoare_triple, bi_hoare;split;intros H.
+  * intros i s s' Pre Heval.
+    eapply H.
+    apply Pre.
+    eapply unroll_n_ceval; apply Heval.
+  * intros s s' Pre Heval.
+    eapply ceval_unroll_n in  Heval.
+    destruct Heval.
+    eapply (H x).
+    apply Pre.
+    assumption.
+Qed.
+
 Lemma while_triple :
   forall (inv: assertion) (var: variant) b c ps l,
-    (forall s1 s2, inv (s1 :: l) /\ beval s1 b = true ->
-                     ceval c s1 ps s2 -> inv (s2 :: l)) ->
+    hoare_triple (fun s => inv (s :: l) /\ beval s b = true)
+                 (fun s' _ => inv (s' :: l)) c ps ->
     hoare_triple (fun s => inv (s :: l))
                 ( fun s' _ => inv (s' :: l) /\ beval s'  b = false )
                 (CWhile b c inv var) ps.
 Proof.
-  intros P var b c ps l Hhoare st st' HP Heval.
-  remember (CWhile b c P var) as original_command eqn:Horig.
-  induction Heval; inversion Horig.
-  * inversion Horig;subst. eauto.
-  * inversion Horig;subst.
+  intros P var b c ps l Hhoare.
+  apply bi_uadruple_quadruple.
+  intros n.
+  induction n;intros st st' HPre Heval.
+  - apply ceval_inf_loop in Heval; now auto.
+  - inversion Heval; subst.
+    inversion H6; subst.
+    eauto.
+    inversion H6; subst.
     eauto.
 Qed.
 
@@ -188,254 +226,72 @@ assumption.
 apply H.
 Qed.
 
-(** ------------------------------ **)
-(** Total correcness               **)
-(** ------------------------------ **)
+Import AexpNotations.
+Import BexpNotations.
+Import ComNotations.
 
-(** Definition of total correcness **)
+Section Loop_Proc.
+  Variable c : com.
+  Variable b: bexp.
 
-Definition total (P : precondition) (Q: postcondition) (c : com) (ps : Psi.psi) : Prop :=
-  forall s ,  P s -> (exists s', ceval c s ps s' /\ Q s' s).
+  Definition w: com :=
+    <[ if {b} then
+         {c};
+         call(1)
+       else
+         skip
+       end ]>.
 
-(** Facts about Hoare Triples **)
+  Definition ps (x': Proc.t) :=
+    if Proc.eqb x' 1 then  w else Psi.empty_psi x'.
 
-Lemma hoare_total (P : precondition) (Q: postcondition) (c : com) (ps : Psi.psi) :
-  hoare_triple P Q c ps ->
- (forall s ,  P s -> (exists s', ceval c s ps s')) ->
- total P Q c ps.
-Proof.
-  intros Hp Hf s HPre.
-  specialize (Hf s HPre).
-  destruct Hf.
-  exists x. split. assumption.
-  apply (Hp _ _ HPre H).
-Qed.
+  Variable invar: assertion.
 
-Lemma total_hoare (P : precondition) (Q: postcondition) (c : com) (ps : Psi.psi) :
- total P Q c ps ->
- hoare_triple P Q c ps.
-Proof.
-  intros Ht s s' HPre Heval.
-  specialize (Ht s HPre).
-  destruct Ht.
-  destruct H.
-  erewrite (ceval_det s _ _ s' x).
-  apply H0.
-  apply Heval.
-  apply H.
-Qed.
+  Variable var: variant.
 
-(** Function for recursive loop unrolling **)
+  Variable l : list sigma.
 
-Fixpoint unroll n b p :=
-  match n with
-  | 0 => CSkip
-  | S n => CSeq (unroll n b p) (CIf b p CSkip)
-  end.
+  Definition pre : precondition := fun s => invar (s :: l).
 
-Lemma total_unroll_c (inv: assertion) (var: variant) b c ps l:
-    total (fun s1 => inv (s1 :: l) /\ beval s1 b = true)
-      (fun s2 s1 => inv (s2 :: l) /\ var s2 < var s1) c ps ->
-    forall n,
-    total (fun s1 => inv (s1 :: l) /\ beval s1 b = true)
-      (fun s2 s1 => inv (s2 :: l) /\ (beval s2 b = true -> var s2 <= var s1 - n))
-      (unroll n b c) ps.
-Proof.
-  intros.
-  induction n;intros s HPre.
-  - exists s. simpl.
-    split.
-    + apply E_Skip.
-    + auto. split. apply HPre. Lia.lia.
-  - specialize (IHn s HPre).
-    destruct IHn.
-    destruct (beval x b) eqn : Hbx.
-    + assert (HPrex: inv (x :: l) /\ beval x b = true).
-      { split;[ apply H0 | assumption ]. }
-      specialize (H x HPrex).
-      destruct H.
-      exists x0;simpl.
-      split.
-      * eapply E_Seq.
-        -- apply H0.
-        -- apply E_IfTrue;[assumption|apply H].
-      * split. apply H. Lia.lia.
-    + exists x;simpl.
-      split.
-      * eapply E_Seq.
-        -- apply H0.
-        -- apply E_IfFalse ;[assumption|apply E_Skip].
-      * split.
-        -- apply H0.
-        -- intros. rewrite H1 in Hbx. inversion Hbx.
-Qed.
+  Definition post : postcondition := fun s' _ => invar (s' :: l) /\ beval s'  b = false.
 
-Lemma unroll_while_while n b c P v ps: forall s s',
-   ceval (CSeq (unroll n b c) (CWhile b c P v)) s ps s' ->
-   ceval (CWhile b c P v) s ps s'.
-Proof.
-  induction n;intros.
-  - simpl in H.
-    inversion H;subst.
-    inversion H2;subst.
-    assumption.
-  - apply IHn.
-    inversion H;subst.
-    inversion H2;subst.
-    eapply E_Seq.
-    apply H3.
-    inversion H8;subst.
-    + eapply E_WhileTrue.
-      apply H10.
-      apply H11.
-      apply H6.
-    + inversion H11;subst.
-      apply H6.
-Qed.
+  Definition cl (f' : Proc.t) : clause :=
+    if (Proc.eqb 1 f')
+    then (pre,post)
+    else Phi.empty_phi f'.
 
-Lemma while_total :
-  forall (inv: assertion) (var: variant) b c ps l,
-    total (fun s1 => inv (s1 :: l) /\ beval s1 b = true)
-          (fun s2 s1 => inv (s2 :: l) /\ var s2 < var s1) c ps ->
-    (forall s1, inv (s1 :: l) -> 0 <= var s1) ->
-    total (fun s => inv (s :: l))
-                (fun s' _ => inv (s' :: l) /\ beval s'  b = false)
-                (CWhile b c inv var) ps.
-Proof.
-  intros P v b c ps l Hhoare Hvariant.
-  apply hoare_total.
-  - apply total_hoare in Hhoare.
-    apply while_triple.
-    apply Hhoare.
-  - intros st HPre.
-    destruct (beval st b) eqn: Hb;[ | exists st; apply E_WhileFalse; assumption].
-    assert (HPreb: P(st :: l) /\ beval st b = true). { split;repeat assumption. }
-    specialize (total_unroll_c _ _ _ _ _ _ Hhoare (v st) st HPreb).
-    intros.
-    destruct H.
-    exists x.
-    apply (unroll_while_while (v st)).
-    eapply E_Seq.
-    apply H.
-    destruct (beval x b) eqn: Hbx.
-    + destruct H.
-      destruct H0.
-      specialize (Hvariant x H0).
-      assert (H2: v x <= v st - v st).
-      { apply H1. reflexivity. }
-      replace (v st - v st) with 0 in H2;[| rewrite Proc.sub_diag;auto].
-      assert (HPrex: P(x :: l) /\ beval x b = true). { split;repeat assumption. }
-      specialize (Hhoare x HPrex).
-      destruct Hhoare.
-      Lia.lia.
-    + apply E_WhileFalse.
-      assumption.
-Qed.
+    Lemma test1 :
+      hoare_triple (fun s => invar (s :: l) /\ beval s b = true)
+        (fun s' _ => invar (s' :: l)) c ps ->
+      hoare_triple (get_pre (cl 1)) (get_post (cl 1)) (CCall 1) ps ->
+      hoare_triple (get_pre (cl 1)) (get_post (cl 1)) (ps 1) ps.
+    Proof.
+      unfold cl;simpl.
+      unfold pre, post.
+      intros.
+      unfold ps;simpl.
+      unfold w.
+      intros s s' HPre Heval.
+      inversion Heval;subst.
+      inversion H8;subst.
+      eapply H0.
+      eapply H.
+      eauto.
+      eauto.
+      auto.
+      inversion H8;subst.
+      auto.
+    Qed.
 
-(** Total correcness for a com with procedure context **)
-
-Definition total_ctx (cl : Phi.phi) (ps: Psi.psi)
-  (P: precondition) (Q: postcondition)  (c: com) :=
-  (forall p, total (get_pre (cl p)) (get_post (cl p)) (CCall p) ps) -> total P Q c ps.
-
-(** Total correcness for a procedure with procedure context **)
-
-Definition total_proc_ctx (var: variant) (cl : Phi.phi) (ps_init :Psi.psi) :=
-  forall v p ps,
-    (forall p, total (fun s => get_pre (cl p) s /\ var s + 1 = v)
-            (get_post (cl p))
-          (CCall p) ps) ->
-    total (fun s => get_pre (cl p) s /\ var s = v) (get_post (cl p))
-      (ps_init p) ps.
-
-(** Defintion of a Hoare Triple with inliner **)
-
-Definition i_total (n: nat)
-  (P: precondition) (Q: postcondition)
-  (c : com) (ps : Psi.psi) : Prop :=
-  forall s ,  P s -> (exists s', ceval (Inline2.k_inliner n c ps) s ps s' /\ Q s' s).
-
-Definition total_proc_ctx_n (n : nat) (var: variant) (cl : Phi.phi) (ps :Psi.psi) :=
-  forall v p,
-    (forall p, total (fun s => get_pre (cl p) s /\ var s + 1 = v - n )
-            (get_post (cl p))
-          (CCall p) ps) ->
-    i_total n (fun s => get_pre (cl p) s /\ var s = v) (get_post (cl p))
-      (CCall p) ps.
-
-Lemma total_proc_ctx_total_proc_ctx_n (var: variant) (cl : Phi.phi) (ps :Psi.psi) :
-  total_proc_ctx var cl ps -> forall n, total_proc_ctx_n n var cl ps.
-Proof.
-  intros H.
-  induction n;intros v p H0 s HPre.
-  - rewrite Proc.sub_0_r in H0.
-    specialize (H v p ps H0 s HPre).
-    destruct H.
-    destruct H.
-    exists x.
-    split;[|auto].
-    apply E_Call.
-    apply H.
-  -
-    assert (Hi: forall p,
-               total (fun s : sigma => get_pre (cl p) s /\ var s + 1 = v )
-                 (get_post (cl p)) (CCall p) ps).
-    { intros p0 s0 HP.
-      specialize (IHn (v - 1) p0).
-      replace (v - 1 - n ) with (v - S n ) in IHn by Lia.lia.
-      destruct HP.
-      apply Proc.add_sub_eq_r in H2.
-      symmetry in H2.
-      assert (HP : get_pre (cl p0) s0 /\ var s0 = v - 1) by auto.
-      specialize (IHn H0 s0 HP).
-      destruct IHn.
-      exists x.
-      destruct H3.
-      apply Inline2.n_inline_ceval_ceval in H3.
-      split; [apply H3 |  apply H4] .
-    }
-    specialize (H v p ps Hi s HPre).
-    destruct H.
-    exists x.
-    split;[|apply H].
-    apply Inline2.ceval_n_inline_ceval.
-    apply E_Call.
-    apply H.
-Qed.
-
-Lemma total_recursive_proc var ps cl:
-    (forall n, total_proc_ctx_n n var cl ps) ->
-   (forall p, total (get_pre (cl p)) (get_post (cl p)) (CCall p) ps).
-Proof.
-  intros.
-  intros s Hpre.
-  assert (H1:  (forall p : Proc.t,
-                   total (fun s0 : sigma => get_pre (cl p) s0 /\ var s0 + 1 = var s - var s)
-                     (get_post (cl p)) (CCall p) ps)).
-  { intros.
-    intros s' HP.
-    Lia.lia.}.
-  assert (HP:  get_pre (cl p) s /\ var s = var s);auto.
-  specialize (H (var s) (var s) p H1 s HP).
-  destruct H.
-  exists x.
-  destruct H.
-  split;[|auto].
-  apply Inline2.n_inline_ceval_ceval in H.
-  eauto.
-Qed.
-
-(** Modular Hoare Triple Verification **)
-
-Theorem recursion_total :
-  forall P Q p var ps cl,
-    total_proc_ctx var cl ps  ->
-    total_ctx cl ps P Q p ->
-    total P Q p ps.
-Proof.
-intros.
-apply H0.
-eapply total_recursive_proc.
-apply total_proc_ctx_total_proc_ctx_n.
-apply H.
-Qed.
+End Loop_Proc.
+ (*    Lemma test2 : *)
+ (*      hoare_triple_proc_ctx cl ps -> *)
+ (*      hoare_triple (fun s => invar (s :: l)) *)
+ (*        ( fun s' _ => invar (s' :: l) /\ beval s'  b = false ) *)
+ (*        (CWhile b c invar var) ps. *)
+ (* Proof. *)
+ (*    intros. *)
+ (*    assert(H1:  forall p, hoare_triple (get_pre (cl p)) (get_post (cl p)) (CCall p) ps). *)
+ (*    apply recursive_proc;assumption. *)
+ (*    specialize (H 1 ps H1). *)
+ (*    intros s s' HPre Heval. *)
