Quadruple.v
@@ -1,4 +1,5 @@
 From Rela Require Import Proc.
+From Rela Require Import Aexp.
 From Rela Require Import Bexp.
 From Rela Require Import Com.
 From Rela Require Import Sigma.
@@ -8,83 +9,17 @@ From Rela Require Import Inliner.
 From Coq Require Import Lia.
 Import Arith.
 
-(* (** Function for loop inlining in Com **) *)
-
-Fixpoint unroll n b p :=
-  match n with
-  | 0 => CWhile BTrue CSkip (fun _ => True) (fun _ => 0)
-  | S n => CIf b  (CSeq p (unroll n b p)) CSkip
-  end.
-
-Lemma inline_n_ceval n p b inv var s ps s':
-  ceval (unroll n b p) s ps s' -> ceval (CWhile b p inv var) s ps s'.
-Proof.
-  generalize dependent s.
-  generalize dependent s'.
-  induction n.
-  * intros.
-    apply ceval_inf_loop in H.
-    contradiction H.
-  * simpl. intros.
-    inversion H;subst.
-    + inversion H7;subst.
-      eapply E_WhileTrue ;[assumption | apply H2 | ].
-      apply IHn;assumption.
-    + inversion H7;subst.
-      apply E_WhileFalse.
-      assumption.
-Qed.
-
-Lemma inline_ceval_S n p b s ps s':
-  ceval (unroll n b p) s ps s' ->
-  forall m, n <= m -> ceval (unroll m b p) s ps s'.
-Proof.
-  intros.
-  generalize dependent s.
-  generalize dependent s'.
-  generalize dependent m.
-  induction n.
-  - intros.
-    apply ceval_inf_loop in H.
-    contradiction H.
-  - destruct m as [| m].
-    + intros. inversion H0.
-    + simpl; intros.
-      inversion H;subst.
-      * inversion H8;subst.
-        apply E_IfTrue;[assumption|].
-        eapply E_Seq ;[apply H3|].
-        apply IHn.
-        Lia.lia.
-        assumption.
-      * apply E_IfFalse;assumption.
-Qed.
-
-Lemma ceval_inline_n p s s' b inv var ps:
-  ceval (CWhile b p inv var) s ps s' -> exists n, ceval (unroll n b p) s ps s'.
-Proof.
-  intros.
-  remember (CWhile b p inv var) as original_command eqn:Horig.
-  induction H; inversion Horig; subst;simpl.
-  * exists 1.
-    apply E_IfFalse;[ apply H | apply E_Skip].
-  * specialize (IHceval2 Horig).
-    destruct IHceval2.
-    exists (S x).
-    apply E_IfTrue;[assumption| eapply E_Seq;eauto ]. 
-Qed.
-
-(** Defintion of relational assertion **)
+(** Defintion of quadruple assertion **)
 
 Definition r_assertion: Type := sigma ->sigma -> Prop.
 
-(** Definition of relational Precondition **)
+(** Definition of quadruple Precondition **)
 
 Definition r_precondition : Type := sigma -> sigma -> Prop.
 
 Definition empty_r_precondition : r_precondition := (fun _ _ => False).
 
-(** Defintion of relational Postcondition **)
+(** Defintion of quadruple Postcondition **)
 
 Definition r_postcondition : Type :=  sigma -> sigma -> sigma -> sigma -> Prop.
 
@@ -93,13 +28,13 @@ Definition empty_r_postcondition :  r_postcondition := (fun _ _ _ _ => True).
 (** Definition of quadruple **)
 
 Definition quadruple (P: r_precondition) (Q: r_postcondition)
-           (c1 c2: com) (ps : Psi.psi) : Prop :=
+  (c1 c2: com) (ps : Psi.psi) : Prop :=
   forall s1 s2 s1' s2', P s1 s2 -> ceval c1 s1 ps s1' -> ceval c2 s2 ps s2' -> Q s1' s2' s1 s2.
 
-(** Definition of a relational properties with inliner for loops **)
+(** Definition of a quadruple properties with inliner for loops **)
 
 Definition i_quadruple (n: nat) (P: r_precondition) (Q: r_postcondition)
-           (c1 c2 : com) (b1 b2: bexp) (ps : Psi.psi) : Prop :=
+  (c1 c2 : com) (b1 b2: bexp) (ps : Psi.psi) : Prop :=
   forall s1 s2 s1' s2', P s1 s2 ->
                    ceval (unroll n b1 c1) s1 ps s1' -> ceval (unroll n b2 c2) s2 ps s2' ->
                    Q s1' s2' s1 s2.
@@ -109,20 +44,20 @@ Lemma qceval_n_inline_loop b1 b2 p1 p2 s1 s2 inv1 inv2 var1 var2 ps s1' s2':
   exists n : nat, ceval (unroll n b1 p1) s1 ps s1' /\ ceval (unroll n b2  p2) s2 ps s2' .
 Proof.
   intros Heval1  Heval2.
-  apply ceval_inline_n in Heval1.
-  apply ceval_inline_n in Heval2.
+  apply ceval_unroll_n in Heval1.
+  apply ceval_unroll_n in Heval2.
   destruct Heval1. destruct Heval2.
   destruct (Nat.max_dec x0 x).
   * exists x0.
     apply PeanoNat.Nat.max_l_iff in e.
     split.
-    eapply inline_ceval_S;[apply H|assumption].
+    eapply unroll_ceval_S;[apply H|assumption].
     apply H0.
   * exists x.
     apply PeanoNat.Nat.max_r_iff in e.
     split.
     apply H.
-    eapply inline_ceval_S;[apply H0|assumption].
+    eapply unroll_ceval_S;[apply H0|assumption].
 Qed.
 
 Lemma i_quadruple_quadruple P Q p1 p2 b1 b2 inv1 inv2 var1 var2 ps:
@@ -133,23 +68,23 @@ Proof.
   - intros n s1 s2 s1' s2' Pre Heval1 Heval2.
     eapply H.
     apply Pre.
-    eapply inline_n_ceval; apply Heval1.
-    eapply inline_n_ceval; apply Heval2.
+    eapply unroll_n_ceval; apply Heval1.
+    eapply unroll_n_ceval; apply Heval2.
   - intros s1 s2 s1' s2' Pre Heval1 Heval2.
     eapply qceval_n_inline_loop in Heval1; [|apply Heval2].
     destruct Heval1. destruct H0.
     eapply H ;eauto.
 Qed.
 
-(** Facts about relational Properties **)
+(** Facts about quadruple Properties **)
 
 Lemma while_quadruple (inv: r_assertion) b1 b2 c1 c2 ps:
   quadruple (fun s1 s2 => inv s1 s2 /\ beval s1 b1 = true /\ beval s2 b2 =  true)
-            (fun s1' s2' _ _ => inv s1' s2' /\ beval s1' b1 = beval s2' b2 ) c1 c2 ps ->
+    (fun s1' s2' _ _ => inv s1' s2' /\ beval s1' b1 = beval s2' b2 ) c1 c2 ps ->
   quadruple ( fun s1 s2 => inv s1 s2 /\ beval s1 b1 = beval s2 b2 )
-            ( fun s1' s2' _ _ => inv s1' s2' /\ beval s1' b1 = false /\ beval s2' b2 = false )
-            (CWhile b1 c1 (fun _=> True) (fun _ => 0))
-            (CWhile b2 c2 (fun _ => True) (fun _ => 0)) ps.
+    ( fun s1' s2' _ _ => inv s1' s2' /\ beval s1' b1 = false /\ beval s2' b2 = false )
+    (CWhile b1 c1 (fun _=> True) (fun _ => 0))
+    (CWhile b2 c2 (fun _ => True) (fun _ => 0)) ps.
 Proof.
   intros Hinv.
   apply i_quadruple_quadruple.
@@ -172,7 +107,7 @@ Proof.
       * rewrite H5,H7 in HP2; now auto.
     + inversion Heval2;subst.
       *  rewrite H5,H7 in HP2.
-        inversion HP2.
+         inversion HP2.
       * inversion H6;subst.
         inversion H8;subst.
         rewrite H5,H7.
@@ -180,19 +115,19 @@ Proof.
 Qed.
 
 Definition bi_quadruple (i: nat) (P: r_precondition) (Q: r_postcondition)
-           (c1 c2 : com) (b1 b2: bexp) (ps : Psi.psi) : Prop :=
+  (c1 c2 : com) (b1 b2: bexp) (ps : Psi.psi) : Prop :=
   forall s1 s2 s1' s2' n m , i = n + m -> P s1 s2 ->
-                   ceval (unroll n b1 c1) s1 ps s1' ->
-                   ceval (unroll m b2 c2) s2 ps s2' ->
-                   Q s1' s2' s1 s2.
+                        ceval (unroll n b1 c1) s1 ps s1' ->
+                        ceval (unroll m b2 c2) s2 ps s2' ->
+                        Q s1' s2' s1 s2.
 
 Lemma qceval_n_b_inline_loop p1 p2 b1 b2 inv1 inv2 var1 var2 s1 s2 ps  s1' s2':
   ceval (CWhile b1 p1 inv1 var1) s1 ps s1' -> ceval (CWhile b2 p2 inv2 var2) s2 ps s2' ->
   exists n m: nat, ceval (unroll n b1 p1) s1 ps s1' /\ ceval (unroll m b2 p2) s2 ps s2' .
 Proof.
   intros Heval1  Heval2.
-  apply ceval_inline_n in Heval1.
-  apply ceval_inline_n in Heval2.
+  apply ceval_unroll_n in Heval1.
+  apply ceval_unroll_n in Heval2.
   destruct Heval1. destruct Heval2.
   exists x. exists x0.
   split.
@@ -208,8 +143,8 @@ Proof.
   * intros i s1 s2 s1' s2' n m Hi Pre Heval1 Heval2.
     eapply H.
     apply Pre.
-    eapply inline_n_ceval; apply Heval1.
-    eapply inline_n_ceval; apply Heval2.
+    eapply unroll_n_ceval; apply Heval1.
+    eapply unroll_n_ceval; apply Heval2.
   * intros s1 s2 s1' s2' Pre Heval1 Heval2.
     eapply qceval_n_b_inline_loop in  Heval1; [| apply Heval2].
     destruct Heval1. destruct H0. destruct H0.
@@ -224,21 +159,21 @@ Definition r_cond: Type := sigma -> sigma -> bool.
 
 Lemma simpl_side_condition b1 b2 L R s1 s2 :
   (beval s1 b1 = beval s2 b2 \/ (beval s1 b1 = true /\ L s1 s2 = true ) \/
-   (beval s2 b2 = true /\ R s1 s2 = true)) ->
+     (beval s2 b2 = true /\ R s1 s2 = true)) ->
   ((beval s1 b1 = true /\ beval s2 b2 = true /\ L s1 s2 = false /\ R s1 s2 = false) \/
-    (beval s1 b1 = false /\ beval s2 b2 = false) \/  (beval s1 b1 = true /\ L s1 s2 = true ) \/
-    (beval s2 b2 = true /\ R s1 s2 = true)).
+     (beval s1 b1 = false /\ beval s2 b2 = false) \/  (beval s1 b1 = true /\ L s1 s2 = true ) \/
+     (beval s2 b2 = true /\ R s1 s2 = true)).
 Proof.
   intros H.
   destruct H.
   * destruct (beval s1 b1) eqn: Hb1.
-    + destruct (L s1 s2) eqn: HL.
-     -  auto.
-     - destruct (R s1 s2) eqn: HR.
-       ** rewrite <- H. auto.
-       ** rewrite <- H. auto.
+  + destruct (L s1 s2) eqn: HL.
+  -  auto.
+  - destruct (R s1 s2) eqn: HR.
+    ** rewrite <- H. auto.
+    ** rewrite <- H. auto.
     + rewrite <- H. auto.
-  * destruct H.
+      * destruct H.
     + destruct H. rewrite H,H0. auto.
     + destruct H. rewrite H,H0. auto.
 Qed.
@@ -253,27 +188,27 @@ Qed.
    b1 /\ not b2 -> X
    not b1 /\ b2 -> Y
 
-*)
+ *)
 
 Lemma while_skedule_quadruple (inv : r_assertion) (L R : r_cond) b1 b2 c1 c2 ps:
   quadruple (fun s1 s2 => inv s1 s2 /\ beval s1 b1 = true /\ beval s2 b2 = true /\
                          L s1 s2 = false /\ R s1 s2 = false)
-            (fun s1' s2' _ _ => inv s1' s2')
-            c1 c2 ps ->
+    (fun s1' s2' _ _ => inv s1' s2')
+    c1 c2 ps ->
   quadruple (fun s1 s2 => inv s1 s2 /\ beval s1 b1 = true  /\ L s1 s2 = true )
-            (fun s1' s2' _ _ => inv s1' s2' )
-            c1 CSkip ps ->
+    (fun s1' s2' _ _ => inv s1' s2' )
+    c1 CSkip ps ->
   quadruple (fun s1 s2 => inv s1 s2 /\ beval s2 b2 = true  /\ R s1 s2 = true)
-            (fun s1' s2' _ _ => inv s1' s2')
-            CSkip c2 ps ->
+    (fun s1' s2' _ _ => inv s1' s2')
+    CSkip c2 ps ->
   (forall s1 s2, inv s1 s2 ->
             beval s1 b1 = beval s2 b2 \/
-            (beval s1 b1 = true /\ L s1 s2 = true ) \/
-            (beval s2 b2 = true /\ R s1 s2 = true)) ->
+              (beval s1 b1 = true /\ L s1 s2 = true ) \/
+              (beval s2 b2 = true /\ R s1 s2 = true)) ->
   quadruple inv
-            ( fun s1' s2' _ _ => inv s1' s2' /\ beval s1' b1 = false /\ beval s2' b2 = false )
-            (CWhile b1 c1 (fun _=> True) (fun _ => 0))
-            (CWhile b2 c2 (fun _ => True) (fun _ => 0)) ps.
+    ( fun s1' s2' _ _ => inv s1' s2' /\ beval s1' b1 = false /\ beval s2' b2 = false )
+    (CWhile b1 c1 (fun _=> True) (fun _ => 0))
+    (CWhile b2 c2 (fun _ => True) (fun _ => 0)) ps.
 Proof.
   intros Hinv1 Hinv2 Hinv3 Hinv.
   apply bi_quadruple_quadruple.
@@ -299,7 +234,7 @@ Proof.
       eapply IHn ;[ apply H1 | | | ].
       eapply Hinv1; [ split;[apply HP| apply H] | apply H2 | apply H3].
       assumption.
-      eapply inline_ceval_S;[apply H12 | Lia.lia].
+      eapply unroll_ceval_S;[apply H12 | Lia.lia].
       rewrite H8 in H; now auto.
       rewrite H6 in H; now auto.
     + destruct H.
@@ -329,36 +264,44 @@ Proof.
            rewrite H6 in H; now auto.
 Qed.
 
-(** Definition of a relational contract **)
+(** Definition of a quadruple contract **)
 
-Definition r_clause : Type := r_precondition * r_postcondition * r_cond * r_cond.
+Definition r_clause : Type := r_precondition * r_postcondition * r_cond * r_cond * r_cond.
 
 Definition empty_clause : r_clause :=
-  (empty_r_precondition, empty_r_postcondition, fun _ _ => true, fun _ _ => true).
+  (empty_r_precondition, empty_r_postcondition, fun _ _ => true, fun _ _ => true, fun _ _ => true).
 
-Definition get_r_pre (an: r_clause) :=
+Definition get_r_pre (an: r_clause) : r_precondition :=
+  let (an,_) := an in
   let (l,_) := an in
   let (l,_) := l in
   let (pre,_) := l in
   pre.
 
-Definition get_r_post (an:r_clause) :=
+Definition get_r_post (an:r_clause) : r_postcondition :=
+  let (an,_) := an in
   let (l,_) := an in
   let (l,_) := l in
   let (_,post) := l in
   post.
 
-Definition get_L (an:r_clause) :=
+Definition get_L (an:r_clause) : r_cond:=
+  let (an,_) := an in
   let (l,_) := an in
   let (_,L) := l in
   L.
 
-Definition get_R (an:r_clause) :=
+Definition get_R (an:r_clause) : r_cond :=
+  let (an,_) := an in
   let (_,R) := an in
   R.
 
-(** Definition of relational contract environments :
-    a map from two procedure name to relational clauses **)
+Definition get_LR (an: r_clause) : r_cond :=
+  let (_,LR) := an in
+  LR.
+
+(** Definition of quadruple contract environments :
+    a map from two procedure name to quadruple clauses **)
 
 Module R_Phi.
 
@@ -368,22 +311,22 @@ Module R_Phi.
 
 End R_Phi.
 
-(**)
+(** Defintion of quadruple with inliner **)
 
 Definition bi_quadruple_fun_2 (i: nat) (P: r_precondition) (Q: r_postcondition)
   (c1 c2 : com) (ps1 ps2 : Psi.psi) : Prop :=
   forall s1 s2 s1' s2' n m, i = n + m -> P s1 s2 ->
-                       ceval c1 s1 (k_inliner_ps n ps1) s1' ->
-                       ceval c2 s2 (k_inliner_ps m ps2) s2' ->
+                       ceval c1 s1 (Inline1.k_inliner_ps n ps1) s1' ->
+                       ceval c2 s2 (Inline1.k_inliner_ps m ps2) s2' ->
                        Q s1' s2' s1 s2.
 
 Lemma qceval_n_b_inline_fun_2 p1 p2 s1 s2 ps1 ps2 s1' s2':
   ceval p1 s1 ps1 s1' ->  ceval p2 s2 ps2 s2' ->
-  exists n m: nat, ceval p1 s1 (k_inliner_ps n ps1) s1' /\ ceval p2 s2 (k_inliner_ps m ps2) s2'.
+  exists n m: nat, ceval p1 s1 (Inline1.k_inliner_ps n ps1) s1' /\ ceval p2 s2 (Inline1.k_inliner_ps m ps2) s2'.
 Proof.
   intros Heval1  Heval2.
-  apply ceval_n_inline_ps in Heval1.
-  apply ceval_n_inline_ps in Heval2.
+  apply Inline1.ceval_n_inline_ps in Heval1.
+  apply Inline1.ceval_n_inline_ps in Heval2.
   destruct Heval1. destruct Heval2.
   exists x. exists x0.
   split.
@@ -392,9 +335,8 @@ Proof.
 Qed.
 
 Definition quadruple_2 (P: r_precondition) (Q: r_postcondition)
-           (c1 c2: com) (ps1 ps2 : Psi.psi) : Prop :=
+  (c1 c2: com) (ps1 ps2 : Psi.psi) : Prop :=
   forall s1 s2 s1' s2', P s1 s2 -> ceval c1 s1 ps1 s1' -> ceval c2 s2 ps2 s2' -> Q s1' s2' s1 s2.
-
 
 Lemma bi_quadruple_quadruple_fun P Q p1 p2 ps1 ps2:
   quadruple_2 P Q p1 p2 ps1 ps2 <-> forall n, bi_quadruple_fun_2 n P Q p1 p2 ps1 ps2.
@@ -403,8 +345,8 @@ Proof.
   * intros i s1 s2 s1' s2' n m Hi Pre Heval1 Heval2.
     eapply H.
     apply Pre.
-    eapply (n_inline_ps_ceval _ _ _ _ _ Heval1).
-    eapply (n_inline_ps_ceval _ _ _ _ _ Heval2).
+    eapply (Inline1.n_inline_ps_ceval _ _ _ _ _ Heval1).
+    eapply (Inline1.n_inline_ps_ceval _ _ _ _ _ Heval2).
   * intros s1 s2 s1' s2' Pre Heval1 Heval2.
     specialize (qceval_n_b_inline_fun_2 _ _ _ _ _ _ _ _  Heval1 Heval2).
     intros Heval. destruct Heval as [n Heval]. destruct Heval as [m Heval].
@@ -418,28 +360,29 @@ Proof.
 Qed.
 
 Definition quadruple_ctx_2 (rcl:R_Phi.r_phi) (ps1 ps2: Psi.psi)
-                            (P: r_precondition) (Q : r_postcondition) (c1 c2:  com) :=
+  (P: r_precondition) (Q : r_postcondition) (c1 c2:  com) :=
   (forall p1 p2, quadruple_2 (get_r_pre (rcl p1 p2))
-                      (get_r_post (rcl p1 p2)) (CCall p1) (CCall p2) ps1 ps2) ->
-      quadruple_2 P Q c1 c2 ps1 ps2.
+              (get_r_post (rcl p1 p2)) (CCall p1) (CCall p2) ps1 ps2) ->
+  quadruple_2 P Q c1 c2 ps1 ps2.
 
 
 Definition quadruple_proc_ctx_2 (rcl : R_Phi.r_phi) (ps_init_1 ps_init_2 :Psi.psi):=
   (forall p1 p2 ps1 ps2,
       quadruple_ctx_2 rcl ps1 ps2 (fun s1 s2 => get_r_pre (rcl p1 p2) s1 s2 /\
-                                             get_L(rcl p1 p2) s1 s2 = false /\
-                                             get_R(rcl p1 p2) s1 s2 = false)
+                                               get_LR(rcl p1 p2) s1 s2 = true /\
+                                               get_L(rcl p1 p2) s1 s2 = false /\
+                                               get_R(rcl p1 p2) s1 s2 = false)
         (get_r_post (rcl p1 p2)) (ps_init_1 p1) (ps_init_2 p2)) /\
-    ( forall p1 p2 ps1 ps2,
+    (forall p1 p2 ps1 ps2,
         quadruple_ctx_2 rcl ps1 ps2 (fun s1 s2 => get_r_pre (rcl p1 p2) s1 s2 /\
-                                               get_L(rcl p1 p2) s1 s2 = true)
+                                                 get_L(rcl p1 p2) s1 s2 = true)
           (get_r_post (rcl p1 p2)) (ps_init_1 p1) (CCall p2)) /\
     (forall p1 p2 ps1 ps2,
         quadruple_ctx_2 rcl ps1 ps2 (fun s1 s2 => get_r_pre (rcl p1 p2) s1 s2 /\
-                                               get_R(rcl p1 p2) s1 s2 = true)
+                                                 get_R(rcl p1 p2) s1 s2 = true)
           (get_r_post (rcl p1 p2)) (CCall p1) (ps_init_2 p2)) /\
     (forall p1 p2 s1 s2,  get_r_pre (rcl p1 p2) s1 s2 ->
-       ((get_L(rcl p1 p2) s1 s2 = false /\ get_R(rcl p1 p2) s1 s2 = false) \/
+                     ((get_LR(rcl p1 p2) s1 s2 = true /\ get_L(rcl p1 p2) s1 s2 = false /\ get_R(rcl p1 p2) s1 s2 = false) \/
                        get_L(rcl p1 p2) s1 s2 = true \/ get_R(rcl p1 p2) s1 s2 = true)).
 
 Lemma ext_r_recursive_proc ps1 ps2 rcl:
@@ -475,10 +418,10 @@ Proof.
       assert (H12: i = n + S m) by lia.
       eapply IHi;[apply H12|apply H5|apply H6|apply H7].
     + split. apply HPre. apply H.
-    + apply n_inline_ps_inline in Heval1.
+    + apply Inline1.n_inline_ps_inline in Heval1.
       apply Heval1.
-    + apply ceval_n_inline_ps_S with (m:= S (S m)) in Heval2 ;[| lia].
-      apply n_inline_ps_inline in Heval2.
+    + apply Inline1.ceval_n_inline_ps_S with (m:= S (S m)) in Heval2 ;[| lia].
+      apply Inline1.n_inline_ps_inline in Heval2.
       apply Heval2.
   - destruct H.
     + eapply H2.
@@ -486,7 +429,7 @@ Proof.
         assert (H12: i = n + S m) by lia.
         eapply IHi;[apply H12|apply H5|apply H6|apply H7].
       * split. apply HPre. apply H.
-      * apply n_inline_ps_inline in Heval1.
+      * apply Inline1.n_inline_ps_inline in Heval1.
         apply Heval1.
       * apply Heval2.
     + eapply H1.
@@ -495,7 +438,7 @@ Proof.
         eapply IHi;[apply H12|apply H5|apply H6|apply H7].
       * split. apply HPre. apply H.
       * apply Heval1.
-      * apply n_inline_ps_inline in Heval2.
+      * apply Inline1.n_inline_ps_inline in Heval2.
         apply Heval2.
 Qed.
 
@@ -506,20 +449,114 @@ Definition quadruple_ctx (rcl:R_Phi.r_phi) (ps: Psi.psi)
 Definition quadruple_proc_ctx (rcl : R_Phi.r_phi) (ps_init :Psi.psi):=
   quadruple_proc_ctx_2 rcl ps_init ps_init.
 
-Theorem recursion_hoare_triple :
+Theorem recursion_quadruple :
   forall P Q p1 p2 ps rcl,
     quadruple_proc_ctx rcl ps  ->
     quadruple_ctx rcl ps P Q p1 p2 ->
     quadruple P Q p1 p2 ps.
 Proof.
-intros.
-apply H0.
-eapply ext_r_recursive_proc.
-apply H.
+  intros.
+  apply H0.
+  apply ext_r_recursive_proc.
+  apply H.
 Qed.
 
-(*Proof the extended rela rule that can use the rule above *)
+Module Test.
+  Definition f1 : Proc.t:= 1.
+  Definition f2 : Proc.t:= 2.
+  Parameter c1 : com.
+  Parameter c2 : com.
+  Parameter b1: bexp.
+  Parameter b2: bexp.
 
-(*Just use the normal termination for the transitivity application, for
+  From Rela Require Import Aexp.
+  From Rela Require Import Bexp.
+
+  Import AexpNotations.
+  Import BexpNotations.
+  Import ComNotations.
+
+  Definition w1: com :=
+    <[ if {b1} then
+         {c1};
+         call(f1)
+       else
+         skip
+       end ]>.
+
+  Definition w2: com :=
+    <[ if {b2} then
+         {c2};
+         call(f2)
+       else
+         skip
+       end ]>.
+
+  Definition ps (x': Proc.t) :=
+    if Proc.eqb x' f1 then  w1 else
+      if Proc.eqb x' f2 then  w2 else Psi.empty_psi x'.
+
+  Parameter invar: r_assertion.
+
+  Definition r_pre : r_precondition := invar.
+
+  Definition r_post : r_postcondition := fun m1 m2 _ _ => invar m1 m2.
+
+  Parameter L: r_cond.
+  Parameter R : r_cond.
+
+  Definition Lc s1 s2 := andb (L s1 s2) (beval s1 b1).
+  Definition Rc s1 s2 := andb (R s1 s2) (beval s2 b2).
+  Definition LR s1 s2 := negb (xorb (beval s1 b1) (beval s2 b2)).
+
+  Definition rcl (f1' f2': Proc.t) : r_clause :=
+    if andb (Proc.eqb f1 f1') (Proc.eqb f2 f2')
+    then (r_pre,r_post, Lc, Rc, LR)
+    else R_Phi.empty_r_phi f1' f2'.
+
+  Lemma test :
+    (forall p1 p2, quadruple_2 (get_r_pre (rcl p1 p2))
+                (get_r_post (rcl p1 p2)) (CCall p1) (CCall p2) ps ps) ->
+    quadruple_proc_ctx rcl ps ->
+    quadruple invar
+      ( fun s1' s2' _ _ => invar s1' s2' /\ beval s1' b1 = false /\ beval s2' b2 = false )
+      (CWhile b1 c1 (fun _=> True) (fun _ => 0))
+      (CWhile b2 c2 (fun _ => True) (fun _ => 0)) ps.
+  Proof.
+    intros H0 H.
+    unfold rcl in H.
+    apply (while_skedule_quadruple _ L R).
+    - unfold quadruple_proc_ctx in H.
+      unfold quadruple_proc_ctx_2 in H.
+      destruct H.
+      clear H1.
+      specialize (H f1 f2 ps ps).
+      unfold quadruple_ctx_2 in H.
+      specialize (H H0).
+      simpl in H.
+      unfold r_pre, r_post, Lc, Rc, LR in H.
+      intros s1 s2 s1' s2' Hpre Heval1 Heval2.
+      specialize (H s1 s2).
+      apply H.
+      split;[apply Hpre|].
+      split.
+      apply Bool.orb_false_iff.
+      split;[apply Hpre|].
+      apply Bool.negb_false_iff.
+      apply Hpre.
+      apply Bool.orb_false_iff.
+      split;[apply Hpre|].
+      apply Bool.negb_false_iff.
+      apply Hpre.
+      unfold ps.
+      simpl.
+      fold ps.
+      unfold w1.
+      apply E_IfTrue.
+      apply Hpre.
+      Search (orb _ (negb _)).
+      (*Proof the extended rela rule that can use the rule above *)
+
+      (*Just use the normal termination for the transitivity application, for
  partial correction use axiom forall f, s, exit s', call f s s'
  and proof the rule from the phd*)
